Prove there are 78498 primes less than one million
Originally the implementation was performing quite poorly due to an
unintended copy-on-modify. Breaking the sieve into pieces before
calling 'mark_multiples' allows us to perform all the modifications
in-place. This reduces execution time from several seconds to 400ms.

Unfortunately the Lean kernel is still too pathetic to be able to
evaluate this, so we have to rely on the 'native_decide' tactic.
As an alternative, this change also proves that the number of primes
found by the sieve will be less than the size of the sieve. That's
not a very tight bound, but adequate for many cases.

FormalVerifyMisc/CodeChef/Template/Primes.lean
@@ -17,6 +17,9 @@ set_option linter.style.commandStart false
 set_option linter.flexible false
 
 def SIEVE_SIZE : ℕ := 1000001
+def SIEVE_SIZE_32 : Int32 := 1000001
+
+@[simp] theorem sieve_size_32_toInt : SIEVE_SIZE_32.toInt = SIEVE_SIZE := rfl
 
 structure Sieve (L : ℕ) where
   -- The sieve - with non-zero values indicating divisors
@@ -54,6 +57,7 @@ structure Sieve (L : ℕ) where
   hdivs_dvd : ∀ j, (jlt : j < divs.size) → divs[j]'(jlt) ≠ 0 →
     (divs[j]'(jlt)).toInt ∣ j ∧
     ∀ y, 1 < y → y ∣ j → (divs[j]'(jlt)).toInt ≤ (y : ℤ)
+  hprimessize : primes.size < i.toInt
 
 theorem sieve_index_toInt_pos {L : ℕ} (S : Sieve L) : 0 < S.i.toInt := lt_trans (by simp) S.hlti
 
@@ -141,29 +145,10 @@ def init_sieve : Sieve SIEVE_SIZE where
     constructor
     · absurd hnz; simp
     · intro y lty ydvd; simp
+  hprimessize := by simp
 
--- Prove that a loop that terminates by showing that 'cur' increases by 'inc'
--- on each iteration and that its absolute value never exceeds 'ub'.
---
--- TODO: This will likely be useful in other file as well
--- consider moving it to a separate file.
-theorem termination_by_increasing_int32 (cur inc : Int32) (ub : ℕ)
-  (curpos : 0 < cur) (incpos : 0 < inc)
-  (curlt : cur.toInt < (ub : ℤ)) (inclt : inc.toInt < (ub : ℤ))
-  (uble : ub ≤ 2^30) :
-  ub - (cur + inc).toInt.natAbs < ub - cur.toInt.natAbs := by
-  have curpos' : 0 < cur.toInt := Int32.lt_iff_toInt_lt.mp curpos
-  have incpos' : 0 < inc.toInt := Int32.lt_iff_toInt_lt.mp incpos
-  rw [int32_toInt_add_of_add_bounds
-    (le_of_lt curpos')
-    (lt_of_lt_of_le curlt (Int.ofNat_le_ofNat_of_le uble))
-    (le_of_lt incpos')
-    (lt_of_lt_of_le inclt (Int.ofNat_le_ofNat_of_le uble))
-    (by simp) (by simp)]
-  rw [← Int.ofNat_natAbs_of_nonneg (le_of_lt curpos')] at curlt
-  apply Nat.sub_lt_sub_left (Int.lt_of_ofNat_lt_ofNat curlt)
-  apply Int.natAbs_lt_natAbs_of_nonneg_of_lt (le_of_lt curpos')
-  exact Int.lt_add_of_pos_right _ incpos'
+theorem init_sieve_size : init_sieve.divs.size = SIEVE_SIZE :=
+  Array.size_replicate
 
 -- The state and constraints required for the 'mark_multiples' loop
 @[ext] structure MarkMultiplesState where
@@ -176,28 +161,46 @@ theorem termination_by_increasing_int32 (cur inc : Int32) (ub : ℕ)
   incle : inc.toInt ≤ A.size
   hAslt : A.size < 2^30
 
-def mark_multiples_state_of_sieve {L : ℕ} (S : Sieve L) : MarkMultiplesState where
-  A := S.divs
-  inc := S.i
-  cur := S.i
+-- For performance reasons we can't pass the sieve itself into 'mark_multiples'
+-- Use this structure to easily repackage and pass the relevant theorems
+structure MMSArgs (L : ℕ) where
+  i : Int32
+  hlti : 1 < i.toInt
+  hile : i.toInt ≤ L
+  hLlt : L < 2^30
+
+def mms_args_of_sieve {L : ℕ} (S : Sieve L) : MMSArgs L where
+  i := S.i
+  hlti := S.hlti
+  hile := S.hile
+  hLlt := S.hLlt
+
+def mark_multiples_state_of_sieve {L : ℕ} (A : Array Int32)
+  (hsize : A.size = L) (args : MMSArgs L)  : MarkMultiplesState where
+  inc := args.i
+  cur := args.i
+  A := A
   incdvd := by simp
-  curpos := sieve_index_toInt_pos S
-  incpos := sieve_index_toInt_pos S
-  incle :=
-    le_of_le_of_eq S.hile (Int.ofNat_inj.mpr S.hsize).symm
-  hAslt := by rw [S.hsize]; exact S.hLlt
+  curpos := by linarith [args.hlti]
+  incpos := by linarith [args.hlti]
+  incle := le_of_le_of_eq args.hile (Int.ofNat_inj.mpr hsize).symm
+  hAslt := by rw [hsize]; exact args.hLlt
 
 @[simp] theorem mark_multiples_state_of_sieve_size {L : ℕ} (S : Sieve L) :
-  (mark_multiples_state_of_sieve S).A.size = S.divs.size := rfl
+  (mark_multiples_state_of_sieve
+    S.divs S.hsize (mms_args_of_sieve S)).A.size = S.divs.size := rfl
 
 @[simp] theorem mark_multiples_state_of_sieve_inc {L : ℕ} (S : Sieve L) :
-  (mark_multiples_state_of_sieve S).inc = S.i := rfl
+  (mark_multiples_state_of_sieve
+    S.divs S.hsize (mms_args_of_sieve S)).inc = S.i := rfl
 
 @[simp] theorem mark_multiples_state_of_sieve_cur {L : ℕ} (S : Sieve L) :
-  (mark_multiples_state_of_sieve S).cur = S.i := rfl
+  (mark_multiples_state_of_sieve
+    S.divs S.hsize (mms_args_of_sieve S)).cur = S.i := rfl
 
 @[simp] theorem mark_multiples_state_of_sieve_array {L : ℕ} (S : Sieve L) :
-  (mark_multiples_state_of_sieve S).A = S.divs := rfl
+  (mark_multiples_state_of_sieve
+    S.divs S.hsize (mms_args_of_sieve S)).A = S.divs := rfl
 
 theorem mark_multiples_state_size_pos (MMS : MarkMultiplesState) : 0 < MMS.A.size := by
   apply Int.lt_of_ofNat_lt_ofNat
@@ -401,13 +404,20 @@ theorem mark_multiples_advance_changed (MMS : MarkMultiplesState)
   rw [getElem_congr_coll (if_pos hz)]
   apply Array.getElem_set_self
 
--- Extract S.divs and mark every entry which is a multiple of S.i
-def mark_multiples {L : ℕ} (S : Sieve L) : MarkMultiplesState :=
-  do_simple_loop (mark_multiples_state_of_sieve S)
+/- Mark every entry of 'A' which is a multiple of args.i
+
+   Originally this function took a Sieve as an argument, but because it isn't
+   given exclusive ownership of that Sieve, the entire array was being copied.
+   This change substantially improves the performance of the algorithm at the
+   cost of slightly more verbose code.
+-/
+def mark_multiples {L : ℕ} (A : Array Int32)
+  (hsize : A.size = L) (args : MMSArgs L) : MarkMultiplesState :=
+  do_simple_loop (mark_multiples_state_of_sieve A hsize args)
 
 -- The size of the marked array is the same as the size of the sieve
 @[simp] theorem mark_multiples_size {L : ℕ} (S : Sieve L) :
-  (mark_multiples S).A.size = S.divs.size := by
+  (mark_multiples S.divs S.hsize (mms_args_of_sieve S)).A.size = S.divs.size := by
   unfold mark_multiples
   rw [← mark_multiples_state_of_sieve_size S]
   apply simple_loop_val_const (_ : MarkMultiplesState) (fun mms ↦ mms.A.size)
@@ -416,8 +426,8 @@ def mark_multiples {L : ℕ} (S : Sieve L) : MarkMultiplesState :=
 
 -- The increment of the marked array is the same as S.i
 @[simp] theorem mark_multiples_inc {L : ℕ} (S : Sieve L) :
-  (mark_multiples S).inc = S.i :=
-  simple_loop_inc_const (mark_multiples_state_of_sieve S)
+  (mark_multiples S.divs S.hsize (mms_args_of_sieve S)).inc = S.i :=
+  @simple_loop_inc_const MarkMultiplesState _ _
 
 -- Prove the equivalence between cur < finish in the SimpleLoopState interface
 -- and the corresponding statement in MarkMultiplesState
@@ -429,10 +439,12 @@ lemma mark_multiples_cur_lt_size_iff_cur_lt_finish (MMS : MarkMultiplesState) :
 -- that were previous marked
 theorem mark_multiples_unchanged_of_marked {L : ℕ} (S : Sieve L) :
   ∀ (j : ℕ), (jpos : 0 < j) → (jlt : j < S.divs.size) → S.divs[j] ≠ 0 →
-  (mark_multiples S).A[j]'(by rwa [mark_multiples_size]) = S.divs[j] := by
+  (mark_multiples S.divs S.hsize (mms_args_of_sieve S)).A[j]'(by
+    rwa [mark_multiples_size]) = S.divs[j] := by
   unfold mark_multiples
   intro j jpos jlt hnz
-  let mms₀ := mark_multiples_state_of_sieve S
+  let mms₀ := mark_multiples_state_of_sieve
+    S.divs S.hsize (mms_args_of_sieve S)
   let prop (mms : MarkMultiplesState) : Prop :=
     (_ : j < mms.A.size) → mms.A[j] ≠ 0 ∧ mms.A[j] = S.divs[j]
   have base : prop mms₀ := by
@@ -453,9 +465,11 @@ theorem mark_multiples_unchanged_of_marked {L : ℕ} (S : Sieve L) :
 -- whose indices are not divisible by 'inc'
 theorem mark_multiples_unchanged_of_not_dvd {L : ℕ} (S : Sieve L) :
   ∀ (j : ℕ), (jpos : 0 < j) → (jlt : j < S.divs.size) → ¬S.i.toInt ∣ (j : ℤ) →
-  (mark_multiples S).A[j]'(by rwa [mark_multiples_size]) = S.divs[j] := by
+  (mark_multiples S.divs S.hsize (mms_args_of_sieve S)).A[j]'(by
+    rwa [mark_multiples_size]) = S.divs[j] := by
   intro j jpos jlt hdvd
-  let mms₀ := mark_multiples_state_of_sieve S
+  let mms₀ := mark_multiples_state_of_sieve
+    S.divs S.hsize (mms_args_of_sieve S)
   let prop (mms : MarkMultiplesState) : Prop :=
     (_ : j < mms.A.size) → ¬mms.inc.toInt ∣ j ∧ mms.A[j] = S.divs[j]
   have base : prop mms₀ := by
@@ -474,10 +488,11 @@ theorem mark_multiples_unchanged_of_not_dvd {L : ℕ} (S : Sieve L) :
 
 -- 'mark_multiples' has no effect on the first entry in the sieve
 theorem mark_multiples_unchanged_of_first {L : ℕ} (S : Sieve L) :
-  (mark_multiples S).A[0]'(
+  (mark_multiples S.divs S.hsize (mms_args_of_sieve S)).A[0]'(
     (mark_multiples_size S) ▸ (sieve_length_pos S)
   ) = S.divs[0]'(sieve_length_pos S) := by
-  let mms₀ := mark_multiples_state_of_sieve S
+  let mms₀ := mark_multiples_state_of_sieve
+    S.divs S.hsize (mms_args_of_sieve S)
   let prop (mms : MarkMultiplesState) : Prop :=
     mms.A[0]'(mark_multiples_state_size_pos mms) = S.divs[0]'(sieve_length_pos S)
   have base : prop mms₀ := by
@@ -495,9 +510,11 @@ theorem mark_multiples_unchanged_of_first {L : ℕ} (S : Sieve L) :
 theorem mark_multiples_changed {L : ℕ} (S : Sieve L) :
   ∀ (j : ℕ), (jpos : 0 < j) → (jlt : j < S.divs.size) →
   S.divs[j] = 0 → S.i.toInt ∣ (j : ℤ) →
-  (mark_multiples S).A[j]'(by rwa [mark_multiples_size]) = S.i := by
+  (mark_multiples S.divs S.hsize (mms_args_of_sieve S)).A[j]'(by
+    rwa [mark_multiples_size]) = S.i := by
   intro j jpos _ hz hdvd
-  let mms₀ := mark_multiples_state_of_sieve S
+  let mms₀ := mark_multiples_state_of_sieve
+    S.divs S.hsize (mms_args_of_sieve S)
   let prop (mms : MarkMultiplesState) : Prop :=
     (_ : j < mms.A.size) → mms.inc.toInt = S.i.toInt →
     (mms.cur.toInt ≤ j → mms.A[j] = 0) ∧
@@ -557,7 +574,8 @@ theorem mark_multiples_changed {L : ℕ} (S : Sieve L) :
 -- after calling mark_multiples
 theorem mark_multiples_marked_of_dvd {L : ℕ} (S : Sieve L) :
   ∀ (j : ℕ), (jpos : 0 < j) → (jlt : j < S.divs.size) → S.i.toInt ∣ (j : ℤ) →
-  (mark_multiples S).A[j]'(by rwa [mark_multiples_size]) ≠ 0 := by
+  (mark_multiples S.divs S.hsize (mms_args_of_sieve S)).A[j]'(by
+    rwa [mark_multiples_size]) ≠ 0 := by
   intro j jpos jlt idvd
   by_cases h : S.divs[j]'jlt = 0
   · rw [mark_multiples_changed S j jpos jlt h idvd]; symm
@@ -581,7 +599,7 @@ lemma sieve_toInt_index_succ {L : ℕ} (S : Sieve L) :
 def advance_sieve_of_entry_eq_zero {L : ℕ} (S : Sieve L)
   (ilt : S.i.toInt.natAbs < S.divs.size)
   (hiz : S.divs[S.i.toInt.natAbs]'ilt = 0) : Sieve L where
-  divs := (mark_multiples S).A
+  divs := (mark_multiples S.divs S.hsize (mms_args_of_sieve S)).A
   primes := S.primes.push S.i
   i := S.i + 1
   hsize := by
@@ -719,6 +737,10 @@ def advance_sieve_of_entry_eq_zero {L : ℕ} (S : Sieve L)
     rename' hmarked => ylt
     apply sieve_marked_of_dvd_of_lt S y j <;> try assumption
     exact (ne_of_lt lty).symm
+  hprimessize := by
+    rw [sieve_toInt_index_succ, Array.size_push]
+    rw [← Int.ofNat_add_ofNat]
+    exact Int.add_lt_add_right S.hprimessize 1
 
 -- Advance the loop which fills out the sieve, in the case where S.divs[i] ≠ 0
 def advance_sieve_of_entry_ne_zero {L : ℕ} (S : Sieve L)
@@ -783,6 +805,10 @@ def advance_sieve_of_entry_ne_zero {L : ℕ} (S : Sieve L)
       absurd h; push_neg
       exact ne_of_lt p'lt
   hdivs_dvd := S.hdivs_dvd
+  hprimessize := by
+    rw [sieve_toInt_index_succ]
+    apply lt_trans _ (Int.add_lt_add_right S.hprimessize 1)
+    simp
 
 -- Combine the two cases into a single advancement function
 def advance_sieve {L : ℕ} (S : Sieve L)
@@ -856,6 +882,19 @@ theorem sieve_of_eratosthenes_index_ge :
   rwa [Sieve.hsize, Int32.toInt_ofNat_of_lt] at this
   unfold SIEVE_SIZE; simp
 
+theorem sieve_of_eratosthenes_index :
+  sieve_of_eratosthenes.i.toInt = SIEVE_SIZE := by
+  have curlt : SimpleLoopState.cur init_sieve < SimpleLoopState.finish init_sieve := by
+    unfold init_sieve SIEVE_SIZE; simp
+  apply le_antisymm _ sieve_of_eratosthenes_index_ge
+  apply Int.le_of_lt_add_one
+  apply lt_of_lt_of_eq (Int32.lt_iff_toInt_lt.mp (simple_loop_index_lt_of_lt init_sieve curlt))
+  rw [simple_loop_state_toInt_finish_add_inc]
+  rw [simple_loop_finish_const, simple_loop_inc_const]; dsimp
+  rw [Int.add_left_inj, init_sieve_size]
+  apply Int32.toInt_ofNat_of_lt
+  unfold SIEVE_SIZE; simp
+
 -- The elements of 'primes' are in-fact prime
 theorem prime_of_mem_primes :
   ∀ n ∈ primes, ∃ (p : ℕ), n.toInt = p ∧ Nat.Prime p := by
@@ -903,5 +942,17 @@ theorem divs_getElem_dvd_and_le :
   apply sieve_marked_of_lt_index S n ltn
   apply lt_of_lt_of_le (Int.ofNat_lt_ofNat_of_lt _) sieve_of_eratosthenes_index_ge
   rwa [← S.hsize]
+
+set_option linter.style.nativeDecide false
+theorem primes_size : primes.size = 78498 := by native_decide
+
+-- Prove that the size of the primes array is less than the sieve size
+-- Note that this result is less precise than 'primes_size' (above)
+-- but doesn't rely on "native decide"
+theorem primes_size_lt_sieve_size : primes.size < SIEVE_SIZE := by
+  unfold primes
+  apply Int.lt_of_ofNat_lt_ofNat
+  apply lt_of_lt_of_eq sieve_of_eratosthenes.hprimessize
+  exact sieve_of_eratosthenes_index
 
 end CodeChef
